Add stuff for day 4

exercises_and_homework_day_3_teacher.v
@@ -19,26 +19,12 @@ Set Asymmetric Patterns.
 (** Some filled in exercises from yesterday; feel free to paste more here. *)
 
 Notation refl := eq_refl.
-Definition sym : forall A (x y : A), x = y -> y = x
-  := fun A x y p
-     => match p in (_ = y) return y = x with
-          | refl => refl
-        end.
-
+Definition sym : forall A (x y : A), x = y -> y = x := eq_sym.
 (** We allow writing [sym p] to mean [sym _ _ _ p] *)
-
 Arguments sym {A x y} p, A x y p.
-
 Definition trans : forall A (x y z : A), x = y -> y = z -> x = z
-  := fun A x y z p
-     => match p in (_ = y) return y = z -> x = z with
-          | refl => fun q => match q in (_ = z) return x = z with
-                               | refl => refl
-                             end
-        end.
-
+  := eq_trans.
 Arguments trans {A x y z} p q, A x y z p q.
-
 Definition J : forall (A : Type) (x : A) (y : A)
                       (H : x = y)
                       (P : forall (y' : A) (H' : x = y'), Type),
@@ -46,17 +32,25 @@ Definition J : forall (A : Type) (x : A) (y : A)
   := fun A x y H P k => match H with
                           | refl => k
                         end.
-
 Arguments J {A} {x} {y} H P _.
+Definition ap : forall A B (f : A -> B) (x y : A), x = y -> f x = f y
+  := fun A B f x y p
+     => match p with
+          | refl => refl
+        end.
+
+Arguments ap {A B} f {x y} p, {A B} f x y p, A B f x y p.
+
 
 (* end hide *)
 
 (** ** Guiding Puzzles *)
 
-(** There are two guiding questions for today:
+(** There are three guiding questions for today:
 
  1. What are (inductive) types?
- 2. What does it mean to say that two inhabitants of a given type are equal? *)
+ 2. What does it mean to say that two inhabitants of a given type are equal?
+ 3. Where is equality under-specified, and how can we extend the patterns we see to fill in these areas? *)
 
 (** *** Puzzle 1: contractibility of based path spaces *)
 
@@ -73,19 +67,21 @@ Definition is_contractible : Type -> Type
 
 (** Puzzle: The following theorem is provable.  Prove it. *)
 
-Definition contractible_pointed : forall (A : Type) (y : A),
-                                    is_contractible { x : A | y = x }
+Definition contractible_pointed
+: forall (A : Type) (y : A),
+    is_contractible { x : A | y = x }
   := admit.
 
 (** Note that [x = y :> T] means [x : T], [y : T], and [x = y].  It is the notation for [@eq T x y].  It is how we write $x =_T y$ #<span class="inlinecode">x =<sub>T</sub> y</span># in Coq. *)
 
 (** Since equals are inter-substitutable, we should be able to prove: *)
 
-Definition contractible_to_UIP : forall (A : Type) (y : A)
-                                        (x : A)
-                                        (p p' : y = x),
-                                   ((x; p) = (x; p') :> { x : A | y = x })
-                                   -> p = p'
+Definition contractible_to_UIP
+: forall (A : Type) (y : A)
+         (x : A)
+         (p p' : y = x),
+    ((x; p) = (x; p') :> { x : A | y = x })
+    -> p = p'
   := admit.
 
 (** But it turns out that we can't prove this.  Why not?  Give both a formal, type theoretic reason (what terms don't typecheck?), and a topological reason. *)
@@ -100,7 +96,8 @@ Definition contractible_to_UIP : forall (A : Type) (y : A)
 
 Section general_classification.
 
-  Definition code_correct_P : forall {A : Type} (code : A -> A -> Type), Type
+  Definition code_correct_P
+  : forall {A : Type} (code : A -> A -> Type), Type
     := admit.
 
   (** We assume we are given a type, a [code], an [encode], and a [decode].  We introduce the assumptions as we get to definitions that should need them. *)
@@ -108,21 +105,24 @@ Section general_classification.
   Context {A : Type} (code : A -> A -> Type)
           (decode' : forall x y, code x y -> x = y).
 
-  Definition decode : forall {x y}, code x y -> x = y
+  Definition decode
+  : forall {x y}, code x y -> x = y
     := admit.
 
   Context (encode : forall x y, x = y -> code x y).
 
-  Definition deencode : forall {x y} (p : x = y),
-                          decode (encode _ _ p) = p
+  Definition deencode
+  : forall {x y} (p : x = y),
+      decode (encode _ _ p) = p
     := admit.
 
   (** For this last one, we'll need the correctness property on codes. *)
 
   Context (code_correct : code_correct_P code).
 
-  Definition endecode : forall {x y} (p : code x y),
-                          encode _ _ (decode p) = p
+  Definition endecode
+  : forall {x y} (p : code x y),
+      encode _ _ (decode p) = p
     := admit.
 
 End general_classification.
@@ -133,8 +133,9 @@ Section sanity_checks.
 
   (** [x = y] should be a valid code *)
 
-  Definition eq_is_valid_code : forall {A : Type},
-                                  code_correct_P (fun x y : A => x = y)
+  Definition eq_is_valid_code
+  : forall {A : Type},
+      code_correct_P (fun x y : A => x = y)
     := admit.
 
   (** If you didn't choose a silly correctness property like [code = (fun x y => x = y)], then your proof should generalize to the following: *)
@@ -154,6 +155,29 @@ Section sanity_checks.
 
 End sanity_checks.
 
+(** *** Puzzle 3 *)
+
+(** Classify the equalities of types.  That is, fill in the following: *)
+
+Definition Type_code
+: forall (x y : Type), Type
+  := admit.
+
+Definition Type_encode
+: forall {x y : Type}, x = y -> Type_code x y
+  := admit.
+
+(** The following are unprovable in Coq, currently.  They are collectively known as the "univalence axiom". *)
+
+Axiom Type_decode
+: forall {x y : Type}, Type_code x y -> x = y.
+Axiom Type_endecode
+: forall {x y : Type} (p : Type_code x y),
+    Type_encode (Type_decode p) = p.
+Axiom Type_deencode
+: forall {x y : Type} (p : x = y),
+    Type_decode (Type_encode p) = p.
+
 (** This was all very abstract.  Let's drill down with some exmples. *)
 
 (** ** Inductive Types *)
@@ -162,15 +186,7 @@ End sanity_checks.
 
 (** An inductive type is specified by introduction and elimination rules; introduction rules tell you how to create inhabitants (elements) of a type, and elimination rules tell you how to use such inhabitants.  Coq generate eliminations rules automatically, but we will try to come up with the first few without peeking. *)
 
-Inductive unit : Type := tt.
-
-Inductive bool : Type := true | false.
-
-(** A notational helper. *)
-
-Add Printing If bool.
-
-(** Now it's your turn to tell me what the constructors should be. *)
+Inductive unit : Set := tt.
 
 (** Coq has special syntax for [nat], so we don't overwrite it. *)
 
@@ -179,6 +195,14 @@ Add Printing If bool.
 (** Inductive Empty_set : Type := ... *)
 
 (** Anecdote: Proving [unit -> Empty_set] (i.e., [True -> False]) by recursion on [unit], if we assume that [False = (True -> True)] *)
+
+(** Any that we don't do in class are homework *)
+
+Inductive bool : Type := true | false.
+
+(** A notational helper. *)
+
+Add Printing If bool.
 
 (** Inductive prod (A B : Type) : Type := ... *)
 
@@ -200,10 +224,12 @@ Example prod_4 := (1, true) : nat * bool.
 
 (** We use curlie braces so that we don't have to pass the arguments explicitly all the time. *)
 
-Definition fst : forall {A B}, A * B -> A
+Definition fst
+: forall {A B}, A * B -> A
 := admit.
 
-Definition snd : forall {A B}, A * B -> B
+Definition snd
+: forall {A B}, A * B -> B
 := admit.
 
 >> *)
@@ -257,11 +283,16 @@ Fail Example dependent_pair_4 :=
 
 (** The projections *)
 
-Definition projT1 : forall {A B}, { a : A | B a } -> A
+(**
+<<
+Definition projT1
+: forall {A B}, { a : A | B a } -> A
   := admit.
 
-Definition projT2 : forall {A B} (x : { a : A | B a}), B (projT1 x)
+Definition projT2
+: forall {A B} (x : { a : A | B a}), B (projT1 x)
   := admit.
+>> *)
 
 (** Notational helpers for the projections *)
 
@@ -276,9 +307,197 @@ Notation "x .2" := (projT2 x) (at level 3, format "x '.2'").
 
 (** Note well: [J] is the eliminator for the equality type. *)
 
+(** *** Provable equalities *)
+
+(** What equalities of types are provable? *)
+
+(** Ask the students to come up with this. *)
+
+
+
+
+
+
+
+
+
+
+
+
+
+
+
+
+
+
+
+
+
+
+
+
+
+
+
+
+
+
+
+
+
+
+
+
+Definition unit_refl : unit = unit
+  := admit.
+
+(** Can you prove this one?  (Take a minute to try on your own.) *)
+
+Inductive unit1 := tt1.
+Inductive unit2 := tt2.
+
+Definition unit12 : unit1 = unit2
+  := admit.
+
+(** Can you prove other ones? *)
+
+(** *** Provable inequalities *)
+
+(** What equalities of types are provably absurd? *)
+
+(** Ask the students to come up with this. *)
+
+
+
+
+
+
+
+
+
+
+
+
+
+
+
+
+
+
+
+
+
+
+
+
+
+Definition unit_Empty_set_absurd : unit = Empty_set -> Empty_set
+  := admit.
+
+(** More generally, when are two types provably different? *)
+
+
+
+
+
+
+
+
+
+
+
+
+
+
+
+
+
+
+
+
+
+
+
+
+
+
+
+
+
+
+
+
+
+
+
+
+
+
+(** *** Isomorphisms *)
+
+(** We can define a notion of isomorphism: *)
+
+Class IsIsomorphism {A B} (f : A -> B)
+  := { iso_inv : B -> A;
+       right_inv : forall x : B, f (iso_inv x) = x;
+       left_inv : forall x : A, iso_inv (f x) = x }.
+
+Arguments iso_inv {A B} f {_} _.
+Arguments right_inv {A B f _ _}, {A B} f {_} _.
+Arguments left_inv {A B f _ _}, {A B} f {_} _.
+
+Record Isomorphic A B
+  := { iso_fun : A -> B;
+       iso_isiso : IsIsomorphism iso_fun }.
+
+Arguments iso_fun {A B} _ _.
+
+(** Let us use an object of type [Isomorphic] as a function: *)
+
+Coercion iso_fun : Isomorphic >-> Funclass.
+
+(** Tell Coq that the function associated to an [Isomorphic] object is always an isomorphism. *)
+
+Existing Instance iso_isiso.
+
+Notation "A <~=~> B" := (Isomorphic A B) (at level 70).
+Notation "A ≅ B" := (Isomorphic A B) (at level 70).
+
+(** We can prove the standard properties about isomorphisms: *)
+
+Definition Isomorphic_refl : forall {A}, A ≅ A
+  := admit.
+
+Definition Isomorphic_inverse : forall {A B}, A ≅ B -> B ≅ A
+  := admit.
+
+Definition Isomorphic_compose : forall {A B C}, A ≅ B -> B ≅ C -> A ≅ C
+  := admit.
+
+(** We would like to prove the last corresponding law: *)
+
+Definition Isomorphic_ap : forall (f : Type -> Type) {A B}, A ≅ B -> f A ≅ f B
+  := admit.
+
+(** But it's not provable!  Here's a counter-example: *)
+
+(** Recall the taboo from earlier; we can't prove equality of two identical types defined separately.  But if we could prove [Isomorphic_ap], then we could prove this! *)
+
+Definition iso_unit2_unit1 : unit2 ≅ unit1
+  := admit.
+
+Definition taboo1 : unit1 = unit2 :> Type
+  := Isomorphic_ap (fun T => T = unit2) iso_unit2_unit1 refl.
+
+(** Ooops!  We'll be coming back to this soon. *)
+
+(** More practice: You can prove the higher groupoid laws about isomorphisms, but it's a bit of a pain. *)
+
+(** Before dealing with the taboo above, let's classify the equality space of isomorphisms. *)
+
 (** ** Equality classification *)
 
-(** We can classify the equality types.  For each type, we come up with a simpler type that represents ("codes for") its equality type.  Then we prove that this type is isomorphic to the given equality type. *)
+(** We can classify the equality types.  For each type, we come up with a simpler type that represents ("codes for") its equality type.  Then we prove that this type is isomorphic to the given equality type.  The exercises here are all to help understand how the encode-decode method works, to build up to function extensionality and univalence, and, for sigma types, to solve the first puzzle.  We'll do them as needed to explain the method; the rest are (optional) homework.  There are more exercises at the bottom of the file. *)
 
 (** *** [unit] *)
 
@@ -302,6 +521,9 @@ Definition unit_deencode : forall {x y} (p : x = y),
   := admit.
 
 
+Definition unit_iso : forall x y : unit, (x = y) ≅ unit_code x y
+  := admit.
+
 (** *** [bool] *)
 
 Definition bool_code : forall (x y : bool), Type
@@ -319,26 +541,6 @@ Definition bool_endecode : forall {x y : bool} (p : bool_code x y),
 
 Definition bool_deencode : forall {x y : bool} (p : x = y),
                              bool_decode (bool_encode p) = p
-  := admit.
-
-
-(** *** [prod] *)
-
-Definition prod_code : forall {A B} (x y : A * B), Type
-  := admit.
-
-Definition prod_encode : forall {A B} {x y : A * B}, x = y -> prod_code x y
-  := admit.
-
-Definition prod_decode : forall {A B} {x y : A * B}, prod_code x y -> x = y
-  := admit.
-
-Definition prod_endecode : forall {A B} {x y : A * B} (p : prod_code x y),
-                             prod_encode (prod_decode p) = p
-  := admit.
-
-Definition prod_deencode : forall {A B} {x y : A * B} (p : x = y),
-                             prod_decode (prod_encode p) = p
   := admit.
 
 
@@ -361,124 +563,6 @@ Definition Empty_set_endecode : forall {x y : Empty_set} (p : Empty_set_code x y
 
 Definition Empty_set_deencode : forall {x y : Empty_set} (p : x = y),
                                   Empty_set_decode (Empty_set_encode p) = p
-  := admit.
-
-
-(** *** [sum] *)
-
-Definition sum_code : forall {A B} (x y : A + B), Type
-  := admit.
-
-Definition sum_encode : forall {A B} {x y : A + B}, x = y -> sum_code x y
-  := admit.
-
-Definition sum_decode : forall {A B} {x y : A + B}, sum_code x y -> x = y
-  := admit.
-
-Definition sum_endecode : forall {A B} {x y : A + B} (p : sum_code x y),
-                             sum_encode (sum_decode p) = p
-  := admit.
-
-Definition sum_deencode : forall {A B} {x y : A + B} (p : x = y),
-                             sum_decode (sum_encode p) = p
-  := admit.
-
-
-(** *** [sigma] (dependent pairs) *)
-
-Definition sigma_code : forall {A B} (x y : { a : A | B a }), Type
-  := admit.
-
-Definition sigma_encode : forall {A B} {x y : { a : A | B a }}, x = y -> sigma_code x y
-  := admit.
-
-Definition sigma_decode : forall {A B} {x y : { a : A | B a }}, sigma_code x y -> x = y
-  := admit.
-
-Definition sigma_endecode : forall {A B} {x y : { a : A | B a }} (p : sigma_code x y),
-                             sigma_encode (sigma_decode p) = p
-  := admit.
-
-Definition sigma_deencode : forall {A B} {x y : { a : A | B a }} (p : x = y),
-                             sigma_decode (sigma_encode p) = p
-  := admit.
-
-
-(** *** [nat] *)
-
-(** Homework: *)
-
-(** Warmup: *)
-
-Definition zero_ne_one : 0 = 1 -> Empty_set
-  := admit.
-
-(** Hint for the above: Use [J]. *)
-
-Definition zero_ne_succ : forall n, 0 = S n -> Empty_set
-  := admit.
-
-Definition nat_code : forall (x y : nat), Type
-  := admit.
-
-Definition nat_encode : forall {x y : nat},
-                                x = y -> nat_code x y
-  := admit.
-
-Definition nat_decode : forall {x y : nat},
-                                nat_code x y -> x = y
-  := admit.
-
-Definition nat_endecode : forall {x y : nat} (p : nat_code x y),
-                                  nat_encode (nat_decode p) = p
-  := admit.
-
-Definition nat_deencode : forall {x y : nat} (p : x = y),
-                                  nat_decode (nat_encode p) = p
-  := admit.
-
-
-(** *** [option] *)
-
-(** Homework: *)
-
-Definition option_code : forall {A} (x y : option A), Type
-  := admit.
-
-Definition option_encode : forall {A} {x y : option A}, x = y -> option_code x y
-  := admit.
-
-Definition option_decode : forall {A} {x y : option A}, option_code x y -> x = y
-  := admit.
-
-Definition option_endecode : forall {A} {x y : option A} (p : option_code x y),
-                             option_encode (option_decode p) = p
-  := admit.
-
-Definition option_deencode : forall {A} {x y : option A} (p : x = y),
-                             option_decode (option_encode p) = p
-  := admit.
-
-
-(** *** [list] *)
-
-(** Homework: *)
-
-Definition list_code : forall {A} (x y : list A), Type
-  := admit.
-
-Definition list_encode : forall {A} {x y : list A}, x = y -> list_code x y
-  := admit.
-
-Definition list_decode : forall {A} {x y : list A}, list_code x y -> x = y
-  := admit.
-
-Definition list_endecode : forall {A} {x y : list A} (p : list_code x y),
-                             list_encode (list_decode p) = p
-  := admit.
-
-Definition list_deencode : forall {A} {x y : list A} (p : x = y),
-                             list_decode (list_encode p) = p
   := admit.
 
 
@@ -513,6 +597,353 @@ Axiom function_endecode : forall {A B} {f g : forall a : A, B a} (p : function_c
                             function_encode (function_decode p) = p.
 Axiom function_deencode : forall {A B} {f g : forall a : A, B a} (p : f = g),
                             function_decode (function_encode p) = p.
+
+
+
+(** *** [sigma] (dependent pairs) *)
+
+(** Homework *)
+
+Definition sigma_code : forall {A B} (x y : { a : A | B a }), Type
+  := admit.
+
+Definition sigma_encode : forall {A B} {x y : { a : A | B a }}, x = y -> sigma_code x y
+  := admit.
+
+Definition sigma_decode : forall {A B} {x y : { a : A | B a }}, sigma_code x y -> x = y
+  := admit.
+
+Definition sigma_endecode : forall {A B} {x y : { a : A | B a }} (p : sigma_code x y),
+                             sigma_encode (sigma_decode p) = p
+  := admit.
+
+Definition sigma_deencode : forall {A B} {x y : { a : A | B a }} (p : x = y),
+                             sigma_decode (sigma_encode p) = p
+  := admit.
+
+
+(** Back to isomorphisms. *)
+
+Definition iso_code : forall {A B} (x y : A ≅ B), Type
+  := admit.
+
+Definition iso_encode : forall {A B} {x y : A ≅ B}, x = y -> iso_code x y
+  := admit.
+
+Definition iso_decode : forall {A B} {x y : A ≅ B}, iso_code x y -> x = y
+  := admit.
+
+Definition iso_endecode : forall {A B} {x y : A ≅ B} (p : iso_code x y),
+                            iso_encode (iso_decode p) = p
+  := admit.
+
+Definition iso_deencode : forall {A B} {x y : A ≅ B} (p : x = y),
+                            iso_decode (iso_encode p) = p
+  := admit.
+
+(** Ooops.  Turns out this isn't provable.  Challenge: Figure out why. *)
+
+(** *** Equivalences *)
+
+(** We can define a slight variation on isomorphisms, called "contractible fibers", which generalizes the notion of injective+surjective.  If you're interested in the various ways of formulating equivalences, Chapter 4 of the HoTT Book (http://homotopytypetheory.org/book/) is an excellent resource. *)
+
+Class Contr (A : Type)
+  := { center : A;
+       contr : forall y, center = y }.
+
+Arguments center A {_}.
+
+Class IsEquiv {A B} (f : A -> B)
+  := Build_IsEquiv : forall b, Contr { a : A | f a = b }.
+
+Record Equiv A B
+  := { equiv_fun : A -> B;
+       equiv_isequiv : IsEquiv equiv_fun }.
+
+Arguments equiv_fun {A B} _ _.
+Arguments equiv_isequiv {A B} _ _.
+
+(** Let us use an object of type [Equiv] as a function: *)
+
+Coercion equiv_fun : Equiv >-> Funclass.
+
+(** Tell Coq that the function associated to an [Equiv] object is
+    always an equivalence. *)
+
+Existing Instance equiv_isequiv.
+
+Notation "A <~> B" := (Equiv A B) (at level 70).
+Notation "A ≃ B" := (Equiv A B) (at level 70).
+
+(** We can prove that an equivalence gives us an isomorphism very easily. *)
+
+Definition iso_of_equiv : forall {A B}, A ≃ B -> A ≅ B.
+Proof.
+  refine admit.
+Defined.
+
+(** We can go the other way with more work. *)
+
+(** Optional Homework: Complete this proof. *)
+
+Definition equiv_of_iso : forall {A B}, A ≅ B -> A ≃ B.
+Proof.
+  refine admit.
+Defined.
+
+(** Now, we prove the following helper lemma, which lets us get the right codes for [Equiv].  We again assume functional extensionality. *)
+
+Definition allpath_contr : forall {A} (x y : Contr A), x = y.
+Proof.
+  refine admit.
+Defined.
+
+Definition allpath_isequiv : forall {A B} (f : A -> B) (e1 e2 : IsEquiv f), e1 = e2.
+Proof.
+  refine admit.
+Defined.
+
+Definition equiv_code : forall {A B} (f g : A ≃ B), Type
+  := admit.
+
+Definition equiv_encode : forall {A B} {f g : A ≃ B}, f = g -> equiv_code f g
+  := admit.
+
+Definition equiv_decode : forall {A B} {f g : A ≃ B}, equiv_code f g -> f = g
+  := admit.
+
+Definition equiv_endecode : forall {A B} {f g : A ≃ B} (p : equiv_code f g),
+                              equiv_encode (equiv_decode p) = p
+  := admit.
+
+Definition equiv_deencode : forall {A B} {f g : A ≃ B} (p : f = g),
+                              equiv_decode (equiv_encode p) = p
+  := admit.
+
+(** Now that we have a "good" type of isomorphism/equivalence (one with the right equality type), we can go back to the question of [Isomorphic_ap]; Recall that we want to prove:
+
+<<
+Definition Isomorphic_ap : forall (f : Type -> Type) {A B}, A ≅ B -> f A ≅ f B.
+>> *)
+
+(** We can prove this by axiomatizing the codes for types: *)
+
+Definition Type_code' : forall (x y : Type), Type
+  := fun x y => x ≃ y.
+
+Definition Type_encode' : forall {x y : Type}, x = y -> Type_code' x y
+  := admit.
+
+(** The following are unprovable in Coq, currently.  They are collectively known as the "univalence axiom". *)
+
+Axiom Type_decode' : forall {x y : Type}, Type_code' x y -> x = y.
+Axiom Type_endecode' : forall {x y : Type} (p : Type_code' x y),
+                         Type_encode' (Type_decode' p) = p.
+Axiom Type_deencode' : forall {x y : Type} (p : x = y),
+                         Type_decode' (Type_encode' p) = p.
+
+Definition Univalence : forall {x y : Type}, IsEquiv (@Type_encode' x y)
+  := admit.
+
+(** *** Homework: Playing with univalence *)
+
+(** Using univalence, we can prove some things. *)
+
+Definition Empty_set_eq : (Empty_set = Empty_set) = unit :> Type
+  := admit.
+
+Definition unit_eq : (unit = unit) = unit :> Type
+  := admit.
+
+Definition bool_eq : (bool = bool) = bool :> Type
+  := admit.
+
+Definition bool_arrow_bool_eq : (bool -> bool) = (bool * bool)%type
+  := admit.
+
+Definition prod_commutes : forall (A B : Type), (A * B = B * A)%type
+  := admit.
+
+(** Challenge: Show, without axioms, that univalence implies functional extensionality: *)
+
+Definition univalence_implies_funext
+: (forall A B, IsEquiv (@Type_encode' A B))
+  -> (forall A B (f g : forall a : A, B a), (forall a, f a = g a) -> f = g)
+  := admit.
+
+(** Exercise 2.17 from the HoTT Book (http://homotopytypetheory.org/book/ - don't worry about reading the book):
+
+  Show that if [A ≃ A'] and [B ≃ B'], then [(A * B) ≃ (A' * B')] in two ways: once using univalence, and once without assuming it. *)
+
+Definition equiv_functor_prod_univalence
+: (forall A B, IsEquiv (@Type_encode A B))
+  -> forall A A' B B',
+       A ≃ A' -> B ≃ B' -> (A * B ≃ A' * B')%type
+  := admit.
+
+Definition equiv_functor_prod_no_univalence
+: forall A A' B B',
+    A ≃ A' -> B ≃ B' -> (A * B ≃ A' * B')%type
+  := admit.
+
+(** Now prove that these two ways are equal *)
+
+Definition equiv_functor_prod_eq
+: forall univalence,
+    equiv_functor_prod_univalence univalence = equiv_functor_prod_no_univalence
+  := admit.
+
+
+
+
+
+
+
+
+
+
+
+
+
+
+
+
+
+
+
+
+
+
+
+
+
+
+
+
+
+
+
+
+
+
+
+
+
+
+
+
+
+(** *** [prod] *)
+
+Definition prod_code : forall {A B} (x y : A * B), Type
+  := admit.
+
+Definition prod_encode : forall {A B} {x y : A * B}, x = y -> prod_code x y
+  := admit.
+
+Definition prod_decode : forall {A B} {x y : A * B}, prod_code x y -> x = y
+  := admit.
+
+Definition prod_endecode : forall {A B} {x y : A * B} (p : prod_code x y),
+                             prod_encode (prod_decode p) = p
+  := admit.
+
+Definition prod_deencode : forall {A B} {x y : A * B} (p : x = y),
+                             prod_decode (prod_encode p) = p
+  := admit.
+
+
+(** *** [sum] *)
+
+Definition sum_code : forall {A B} (x y : A + B), Type
+  := admit.
+
+Definition sum_encode : forall {A B} {x y : A + B}, x = y -> sum_code x y
+  := admit.
+
+Definition sum_decode : forall {A B} {x y : A + B}, sum_code x y -> x = y
+  := admit.
+
+Definition sum_endecode : forall {A B} {x y : A + B} (p : sum_code x y),
+                             sum_encode (sum_decode p) = p
+  := admit.
+
+Definition sum_deencode : forall {A B} {x y : A + B} (p : x = y),
+                             sum_decode (sum_encode p) = p
+  := admit.
+
+
+(** *** [nat] *)
+
+(** Warmup: *)
+
+Definition zero_ne_one : 0 = 1 -> Empty_set
+  := admit.
+
+(** Hint for the above: Use [J]. *)
+
+Definition zero_ne_succ : forall n, 0 = S n -> Empty_set
+  := admit.
+
+Definition nat_code : forall (x y : nat), Type
+  := admit.
+
+Definition nat_encode : forall {x y : nat},
+                                x = y -> nat_code x y
+  := admit.
+
+Definition nat_decode : forall {x y : nat},
+                                nat_code x y -> x = y
+  := admit.
+
+Definition nat_endecode : forall {x y : nat} (p : nat_code x y),
+                                  nat_encode (nat_decode p) = p
+  := admit.
+
+Definition nat_deencode : forall {x y : nat} (p : x = y),
+                                  nat_decode (nat_encode p) = p
+  := admit.
+
+
+(** *** [option] *)
+
+Definition option_code : forall {A} (x y : option A), Type
+  := admit.
+
+Definition option_encode : forall {A} {x y : option A}, x = y -> option_code x y
+  := admit.
+
+Definition option_decode : forall {A} {x y : option A}, option_code x y -> x = y
+  := admit.
+
+Definition option_endecode : forall {A} {x y : option A} (p : option_code x y),
+                             option_encode (option_decode p) = p
+  := admit.
+
+Definition option_deencode : forall {A} {x y : option A} (p : x = y),
+                             option_decode (option_encode p) = p
+  := admit.
+
+
+(** *** [list] *)
+
+Definition list_code : forall {A} (x y : list A), Type
+  := admit.
+
+Definition list_encode : forall {A} {x y : list A}, x = y -> list_code x y
+  := admit.
+
+Definition list_decode : forall {A} {x y : list A}, list_code x y -> x = y
+  := admit.
+
+Definition list_endecode : forall {A} {x y : list A} (p : list_code x y),
+                             list_encode (list_decode p) = p
+  := admit.
+
+Definition list_deencode : forall {A} {x y : list A} (p : x = y),
+                             list_decode (list_encode p) = p
+  := admit.
+
 
 (** **** Homework: mere propositions *)
 
